\begin{answer}
\begin{eqnarray*}
p(t^{(i)}=1\mid y^{(i)} = 1, x^{(i)}) =\frac{p(y^{(i)} = 1\mid t^{(i)}=1, x^{(i)})p(t^{(i)}=1, x^{(i)})}{p(y^{(i)} = 1, x^{(i)})}\\
=\frac{p(y^{(i)} = 1\mid t^{(i)}=1, x^{(i)})p(t^{(i)}=1, x^{(i)})}{p(y^{(i)} = 1\mid t^{(i)}=1, x^{(i)})p(t^{(i)}=1, x^{(i)})+p(y^{(i)} = 1\mid t^{(i)}=0, x^{(i)})p(t^{(i)}=0, x^{(i)})}\\
=\frac{p(y^{(i)} = 1\mid t^{(i)}=1, x^{(i)})p(t^{(i)}=1, x^{(i)})}{p(y^{(i)} = 1\mid t^{(i)}=1, x^{(i)})p(t^{(i)}=1, x^{(i)})}\\
=1
\end{eqnarray*}
\end{answer}
