\begin{answer}
\begin{align*}
h(x^{(i)})&=p(y^{(i)}=1\mid x^{(i)})\\
&=p(y^{(i)}=1\mid t^{(i)}=0,x^{(i)})\cdot p(t^{(i)}=0,x^{(i)})+p(y^{(i)}=1\mid t^{(i)}=1,x^{(i)})\cdot p(t^{(i)}=1,x^{(i)})\\
&=\alpha\cdot p(t^{(i)}=1,x^{(i)})
\end{align*}
When $y^{(i)}=1$,
\begin{align*}
h(x^{(i)})&=\alpha\cdot p(t^{(i)}=1\mid y^{(i)}=1,x^{(i)})\\
&=\alpha
\end{align*}
When $y^{(i)}=0$,
\begin{align*}
h(x^{(i)})&=\alpha\cdot p(t^{(i)}=1\mid y^{(i)}=0,x^{(i)})=\alpha\\
&=\alpha\cdot\frac{p(t^{(i)}=1 \cap y^{(i)}=0,x^{(i)})}{p(y^{(i)}=0,x^{(i)})}\\
&=\alpha\cdot\frac{0}{p(y^{(i)}=0,x^{(i)})}\\
&=0
\end{align*}
\end{answer}
