\begin{answer}
\begin{eqnarray*}
p(y = 1\mid x; \phi, \mu_0, \mu_1, \Sigma)
=\frac{p(x \mid y = 1;\mu_0, \mu_1, \Sigma)p(y=1;\phi)}{p(x;\phi, \mu_0, \mu_1, \Sigma)}\\
=\frac{p(x \mid y = 1;\mu_0, \mu_1, \Sigma)p(y=1;\phi)}{p(x \mid y = 0;\mu_0, \mu_1, \Sigma)p(y=0;\phi)+p(x \mid y = 1;\mu_0, \mu_1, \Sigma)p(y=1;\phi)}\\
=\frac{\frac{1}{(2\pi)^{\di/2} |\Sigma|^{1/2}}\exp\left(-\frac{1}{2}(x-\mu_1)^T \Sigma^{-1} (x-\mu_1) \right)\phi}{\frac{1}{(2\pi)^{\di/2} |\Sigma|^{1/2}}\exp\left(-\frac{1}{2}(x-\mu_{0})^T \Sigma^{-1} (x-\mu_{0})\right)(1-\phi)+\frac{1}{(2\pi)^{\di/2} |\Sigma|^{1/2}}\exp\left(-\frac{1}{2}(x-\mu_1)^T \Sigma^{-1} (x-\mu_1) \right)\phi}\\
=\frac{\exp\left(-\frac{1}{2}(x-\mu_1)^T \Sigma^{-1} (x-\mu_1) \right)\phi}{\exp\left(-\frac{1}{2}(x-\mu_{0})^T \Sigma^{-1} (x-\mu_{0})\right)(1-\phi)+\exp\left(-\frac{1}{2}(x-\mu_1)^T \Sigma^{-1} (x-\mu_1) \right)\phi}\\
=\frac{1}{\frac{\exp\left(-\frac{1}{2}(x-\mu_{0})^T \Sigma^{-1} (x-\mu_{0})\right)(1-\phi)}{\exp\left(-\frac{1}{2}(x-\mu_1)^T \Sigma^{-1} (x-\mu_1) \right)\phi}+1}\\
=\frac{1}{\frac{(1-\phi)}{\phi}\exp\left(-\frac{1}{2}(x-\mu_{0})^T \Sigma^{-1} (x-\mu_{0})-(-\frac{1}{2}(x-\mu_1)^T \Sigma^{-1} (x-\mu_1))\right)+1}\\
=\frac{1}{\exp\left(\log(\frac{(1-\phi)}{\phi})\right)\exp\left((\mu_0-\mu_1)^T\Sigma^{-1}x+\frac{1}{2}(\mu_1^T\Sigma^{-1}\mu_1-\mu_0^T\Sigma^{-1}\mu_0)\right)+1}\\
=\frac{1}{\exp\left((\mu_0-\mu_1)^T\Sigma^{-1}x+\frac{1}{2}(\mu_1^T\Sigma^{-1}\mu_1-\mu_0^T\Sigma^{-1}\mu_0)+\log(\frac{(1-\phi)}{\phi})\right)+1}\\
= \frac{1}{1 + \exp(-(\theta^T x + \theta_0))}
\end{eqnarray*}
${\theta^T=-(\mu_0-\mu_1)^T\Sigma^{-1}}$\\
${\theta_0=-((\mu_1^T\Sigma^{-1}\mu_1-\mu_0^T\Sigma^{-1}\mu_0)+\log(\frac{(1-\phi)}{\phi}))}$
\end{answer}
