\begin{answer}
  \begin{align*}
\ell(\phi, \mu_{0}, \mu_1, \Sigma) &= \log \prod_{i=1}^\nexp p(x^{(i)} , y^{(i)};\phi, \mu_{0}, \mu_1, \Sigma) \\
&= \log \prod_{i=1}^\nexp p(x^{(i)} | y^{(i)}; \mu_{0}, \mu_1, \Sigma) p(y^{(i)};\phi) \\
&= \sum_{i=1}^\nexp \log \left( p(x^{(i)} | y^{(i)}; \mu_{0}, \mu_1, \Sigma) \right) + \sum_{i=1}^\nexp \log\left( p(y^{(i)};\phi)\right)
  \end{align*}
  \begin{align*}
\frac{\partial\ell}{\partial\phi}&=\frac{\partial}{\partial\phi}\sum_{i=1}^\nexp \log \left( p(y^{(i)};\phi)\right)\\
&=\frac{\partial}{\partial\phi}\sum_{i=1}^\nexp \log \left(\phi^{y^{(i)}} (1-\phi)^{(1-y^{(i)})} \right)\\
&=\frac{\partial}{\partial\phi}\sum_{i=1}^\nexp \left( y^{(i)}\log \phi+(1-y^{(i)})\log (1-\phi) ) \right)\\
&=\sum_{i=1}^\nexp \left( \frac{y^{(i)}}{\phi}-\frac{(1-y^{(i)})}{(1-\phi)}  \right)\\
&=\sum_{i=1}^\nexp \left( (1-\phi)y^{(i)}-\phi(1-y^{(i)})  \right)\\
&=\sum_{i=1}^\nexp \left( y^{(i)}-\phi y^{(i)}-\phi+\phi y^{(i)}  \right)\\
&=\sum_{i=1}^\nexp \left( y^{(i)}-\phi \right)\\
&=\sum_{i=1}^\nexp y^{(i)}-\nexp\phi=0
  \end{align*}
  \begin{align*}
\phi=\frac{1}{\nexp}\sum_{i=1}^\nexp y^{(i)}=\frac{1}{\nexp} \sum_{i=1}^\nexp 1\{y^{(i)} = 1\}
  \end{align*}
  \begin{align*}
\frac{\partial\ell}{\partial\mu_{0}}&=\frac{\partial}{\partial\mu_{0}}\sum_{i=1}^\nexp \log \left( p(x^{(i)} | y^{(i)}; \mu_{0}, \mu_1, \Sigma) \right)\\
&=\frac{\partial}{\partial\mu_{0}}\sum_{i=1}^\nexp \log \left(\frac{1}{(2\pi)^{\di/2} |\Sigma|^{1/2}}\exp\left(-\frac{1}{2}(x^{(i)}-\mu_{0})^T \Sigma^{-1} (x^{(i)}-\mu_{0})\right) \right)\\
&=\frac{\partial}{\partial\mu_{0}}\left(\sum_{i=1}^\nexp \log \left(\frac{1}{(2\pi)^{\di/2} |\Sigma|^{1/2}}\right)+\sum_{i=1}^\nexp \log\left(\exp\left(-\frac{1}{2}(x^{(i)}-\mu_{0})^T \Sigma^{-1} (x^{(i)}-\mu_{0})\right) \right)\right)\\
&=\frac{\partial}{\partial\mu_{0}}\sum_{i=1}^\nexp \left(-\frac{1}{2}(x^{(i)}-\mu_{0})^T \Sigma^{-1} (x^{(i)}-\mu_{0})\right) \\
&=\sum_{i=1}^\nexp \left(-\frac{1}{2}(-2)(x^{(i)}-\mu_{0})^T \Sigma^{-1}1\{y^{(i)} = 0\}\right) \\
&=\Sigma^{-1}\sum_{i=1}^\nexp \left((x^{(i)}-\mu_{0})^T 1\{y^{(i)} = 0\}\right) \\
&=\Sigma^{-1}\left(\sum_{i=1}^\nexp  1\{y^{(i)} = 0\}x^{(i)}-\sum_{i=1}^\nexp 1\{y^{(i)} = 0\}\mu_{0}\right) \\
&=\Sigma^{-1}\left(\sum_{i=1}^\nexp 1\{y^{(i)} = 0\}x^{(i)}-\mu_{0}\sum_{i=1}^\nexp 1\{y^{(i)} = 0\}\right)=0
  \end{align*}
  \begin{align*}
\mu_0=\frac{\sum_{i=1}^\nexp 1\{y^{(i)} = {0}\} x^{(i)}}{\sum_{i=1}^\nexp1\{y^{(i)} = {0}\}}
  \end{align*}
  \begin{align*}
\frac{\partial\ell}{\partial\mu_{1}}=\Sigma^{-1}\left(\sum_{i=1}^\nexp 1\{y^{(i)} = 1\}x^{(i)}-\mu_{1}\sum_{i=1}^\nexp 1\{y^{(i)} = 1\}\right)=0
  \end{align*}
  \begin{align*}
\mu_1=\frac{\sum_{i=1}^\nexp 1\{y^{(i)} = {1}\} x^{(i)}}{\sum_{i=1}^\nexp1\{y^{(i)} = {1}\}}
  \end{align*}
  \begin{align*}
\frac{\partial\ell}{\partial\Sigma^{-1}}&=\frac{\partial}{\partial\Sigma^{-1}}\sum_{i=1}^\nexp \log \left( p(x^{(i)} | y^{(i)}; \mu_{0}, \mu_1, \Sigma) \right)\\
&=\frac{\partial}{\partial\Sigma^{-1}}\sum_{i=1}^\nexp \log \left(\frac{1}{(2\pi)^{\di/2} |\Sigma|^{1/2}}\exp\left(-\frac{1}{2}(x^{(i)}-\mu_{y^{(i)}})^T \Sigma^{-1} (x^{(i)}-\mu_{y^{(i)}})\right) \right)\\
&=\frac{\partial}{\partial\Sigma^{-1}}\left(\sum_{i=1}^\nexp \log \left(\frac{1}{(2\pi)^{\di/2}}\right)+\sum_{i=1}^\nexp \log \left(\frac{1}{|\Sigma|^{1/2}}\right)+\sum_{i=1}^\nexp \log\left(\exp\left(-\frac{1}{2}(x^{(i)}-\mu_{y^{(i)}})^T \Sigma^{-1} (x^{(i)}-\mu_{y^{(i)}})\right) \right)\right)\\
&=\frac{\partial}{\partial\Sigma^{-1}}\left(\frac{1}{2}\sum_{i=1}^\nexp \log|\Sigma^{-1}|+\sum_{i=1}^\nexp \left(-\frac{1}{2}(x^{(i)}-\mu_{y^{(i)}})^T \Sigma^{-1} (x^{(i)}-\mu_{y^{(i)}})\right)\right)\\
&=\left(\frac{\nexp}{2}\Sigma+\sum_{i=1}^\nexp \left(-\frac{1}{2}(x^{(i)}-\mu_{y^{(i)}})^T(x^{(i)}-\mu_{y^{(i)}})\right)\right)=0
  \end{align*}
  \begin{align*}
\Sigma=\frac{1}{\nexp} \sum_{i=1}^\nexp (x^{(i)} - \mu_{y^{(i)}}) (x^{(i)} -\mu_{y^{(i)}})^T
  \end{align*}
\end{answer}
