\begin{answer}
\begin{eqnarray*}
\frac{\partial}{\partial \eta} \int p(y;\eta) dy = \int \frac{\partial}{\partial \eta} p(y;\eta) dy\\
=\int \frac{\partial}{\partial \eta} \left(b(y)\exp(\eta y - a(\eta))\right) dy\\
=\int\left(y-\frac{\partial}{\partial \eta}a(\eta)\right)\left(b(y)\exp(\eta y - a(\eta))\right) dy\\
=\int\left(y-\frac{\partial}{\partial \eta}a(\eta)\right)p(y;\eta)dy\\
=\int\left(y\cdot p(y;\eta)-\left(\frac{\partial}{\partial \eta}a(\eta)\right)p(y;\eta)\right)dy\\
=\int y\cdot p(y;\eta)dy-\int\left(\frac{\partial}{\partial \eta}a(\eta)\right)p(y;\eta) dy\\
=\mathbb{E}[Y; \eta]-\frac{\partial}{\partial \eta}a(\eta) \int p(y;\eta) dy\\
=\mathbb{E}[Y; \eta]-\frac{\partial}{\partial \eta}a(\eta)=0
\\
\mathbb{E}[Y; \eta]=\frac{\partial}{\partial \eta}a(\eta)
\end{eqnarray*}
\end{answer}
