\begin{answer}
\begin{enumerate}
\item 
Is a kernel, because:
\begin{align*}
\textbf{y}^TK\textbf{y}&=\textbf{y}^T(K_1+K_2)\textbf{y}\\
&=\textbf{y}^TK_1\textbf{y}+\textbf{y}^TK_2\textbf{y}
\end{align*}
\begin{align*}
\textbf{y}^TK_1\textbf{y}\geq0,\textbf{y}^TK_2\textbf{y}\geq0\Rightarrow \textbf{y}^TK\textbf{y}=\textbf{y}^TK_1\textbf{y}+\textbf{y}^TK_2\textbf{y}\geq0
\end{align*}
\item 
Not a kernel, counter-example:
\begin{align*}
K_1=
   \begin{bmatrix} 
   1&0\\ 
   0&1\\ 
   \end{bmatrix},
K_2=
   \begin{bmatrix} 
   2&0\\ 
   0&2\\ 
   \end{bmatrix}\Rightarrow
K=
   \begin{bmatrix} 
   -1&0\\ 
   0&-1\\ 
   \end{bmatrix} \text{Which is not positive semidefinite}
\end{align*}
\item 
Is a kernel, because:
\begin{align*}
\textbf{y}^TK\textbf{y}&=\textbf{y}^TaK_1\textbf{y}\\
&=a\textbf{y}^TK_1\textbf{y}
\end{align*}
\begin{align*}
\textbf{y}^TK_1\textbf{y}\geq0\Rightarrow\textbf{y}^TK\textbf{y}=a\textbf{y}^TK_1\textbf{y}\geq0
\end{align*}
\item 
Not a kernel, because:
\begin{align*}
\textbf{y}^TK\textbf{y}&=\textbf{y}^T-aK_1\textbf{y}\\
&=-a\textbf{y}^TK_1\textbf{y}
\end{align*}
\begin{align*}
\textbf{y}^TK_1\textbf{y}\geq0\Rightarrow\textbf{y}^TK\textbf{y}=-a\textbf{y}^TK_1\textbf{y}\leq0
\end{align*}
\item 
\item 
\item 
\item 
\end{enumerate}
\end{answer}
