\begin{answer}
\begin{eqnarray*}
\frac{\partial}{\partial\theta_{j}}\left(\log p(y^{(i)} | x^{(i)}; \theta)\right)=\frac{\partial}{\partial\theta_{j}}\left(\log\left(\frac{1}{y^{(i)}!}\cdot\exp\left((\theta^{T}x^{(i)})^{T}y^{(i)}-e^{\theta^{T}x^{(i)}}\right)\right)\right)\\
=\frac{\partial}{\partial\theta_{j}}\left((\theta^{T}x^{(i)})^{T}y^{(i)}-e^{\theta^{T}x^{(i)}}-\log(y^{(i)}!)\right)\\
=\frac{\partial}{\partial\theta_{j}}\left(\left(\sum_{k}\theta_{k}x_{k}^{(i)}\right)y^{(i)}-e^{\sum_{k}\theta_{k}x_{k}^{(i)}}\right)\\
=x_{j}^{(i)}y^{(i)}-x_{j}^{(i)}\cdot e^{\sum_{k}\theta_{k}x_{k}^{(i)}}\\
=x_{j}^{(i)}(y^{(i)}-e^{\theta^{T}x^{(i)}}) 
\end{eqnarray*}
\begin{eqnarray*}
\theta_{j}:=\theta_{j}+\alpha\frac{\partial}{\partial\theta_{j}}l(\theta)\\
=\theta_{j}+\alpha\cdot x_{j}^{(i)}(y^{(i)}-e^{\theta^{T}x^{(i)}}) 
\end{eqnarray*}
\end{answer}
