\begin{answer}
\begin{enumerate}
\item
I will represent $\theta^{(i)}$ in terms of low-dimentional  $\beta^{(i)}$.
\begin{align*}
\theta^{(i)}=\beta^{(i)}\phi(x^{(i)})
\end{align*}
\begin{align*}
\theta^{(0)}=\vec{0}\Rightarrow\beta^{(0)}=\vec{0}
\end{align*}
\item
\begin{align*}
h_{\theta^{(i)}}(x^{(i+1)})&= g({\theta^{(i)}}^T \phi(x^{(i+1)}))\\
&=g(\beta^{(i)}\phi(x^{(i+1)})^T\phi(x^{(i+1)})))\\
&=g(\beta^{(i)}K(x^{(i+1)},x^{(i+1)})))
\end{align*}
I can predict faster using a kernel function.
\item
\begin{align*}
\theta^{(i+1)}&:=	  \theta^{(i)} + \alpha(y^{(i+1)} - h_{\theta^{(i)}}(\phi(x^{(i+1)})))\phi(x^{(i+1)})\\
&=\theta^{(i)} + \alpha(y^{(i+1)} -g(\theta^{(i)^T}\phi(x^{(i+1)})))\phi(x^{(i+1)})\\
&=\beta^{(i)}\phi(x^{(i+1)}) + \alpha(y^{(i+1)} -g(\beta^{(i)}\phi(x^{(i+1)})^T\phi(x^{(i+1)})))\phi(x^{(i+1)})\\
&=(\beta^{(i)}+ \alpha(y^{(i+1)} -g(\beta^{(i)}K(x^{(i+1)},x^{(i+1)}))))\phi(x^{(i+1)})\\
&=\beta^{(i+1)}\phi(x^{(i+1)})
\end{align*}
\begin{align*}
\beta^{(i+1)}&:=\beta^{(i)}+ \alpha(y^{(i+1)} -g(\beta^{(i)}K(x^{(i+1)},x^{(i+1)})))
\end{align*}
\end{enumerate}
\end{answer}
